\section{4-fold Rotational Symmetry}\label{sec:appendix:rotations:4foldRot}

For a rotation of $\theta=\frac{\pi}{2}$, the transformation matrix is given by

\begin{equation}\label{eq:pi/2RotationMatrix}
	R(\theta=\frac{\pi}{2})_{i,j} =
	\begin{bmatrix}
		0 & -1 & 0\\ 
		1 & 0 & 0\\ 
		0 & 0 & 1
	\end{bmatrix}
\end{equation}
We apply the rotation to $\chi_{ijk}$ given in equation~\ref{eq:background:NonlinearOptics:shgP:chiFull}, as in equation~\ref{eq:background:NonlinearOptics:rotation:RotateChi}, giving
\begin{equation}\label{eq:ChiFull4fold}
	\chi_{ijk}^{\prime} =
	\begin{bmatrix}
		-\chi_{yyy} & -\chi_{yxx} & -\chi_{yzz} & -\chi_{yxz} & -\chi_{yzx} & \chi_{yzy} & \chi_{yyz} & \chi_{yyx} & \chi_{yxy}\\ 
		\chi_{xyy} & \chi_{xxx} & \chi_{xzz} & \chi_{xxz} & \chi_{xzx} & -\chi_{xzy} & -\chi_{xyz} & -\chi_{xyx} & -\chi_{xxy}\\ 
		\chi_{zyy} & \chi_{zxx} & \chi_{zzz} & \chi_{zxz} & \chi_{zzx} & -\chi_{zzy} & -\chi_{zyz} & -\chi_{zyx} & -\chi_{zxy}
	\end{bmatrix}
\end{equation}
By enforcing the symmetry $\chi_{ijk}^{\prime}=\chi_{ijk}$, we find that 7 independent components remain, leaving
\begin{equation}\label{eq:4foldChi}
	\chi^{(2)}_{ijk} =
	\begin{bmatrix}
		0 & 0 & 0 & \chi_{xyz} & \chi_{xzy} & \chi_{xzx} & \chi_{xxz} & 0 & 0\\ 
		0 & 0 & 0 & \chi_{yyz} & \chi_{yzy} & \chi_{yzx} & \chi_{yxz} & 0 & 0\\ 
		\chi_{zxx} & \chi_{zyy} & \chi_{zzz} & 0 & 0 & 0 & 0 & \chi_{zxy} & \chi_{zyx}
	\end{bmatrix}
\end{equation}
with dependencies given by
\begin{equation}\label{eq:4foldDependancies}
\begin{split}
	&\chi_{xyz} = -\chi_{yxz}, \chi_{xzy} = -\chi_{yzx}, \chi_{xzx} = \chi_{yzy} \\
	&\chi_{xxz} = \chi_{yyz}, \chi_{zxx} = \chi_{zyy}, \chi_{zxy} = -\chi_{zyx} \\
	&\chi_{zzz}
\end{split}
\end{equation}
Applying permutation symmetry leaves the reduced tensor as
\begin{equation}\label{eq:Reduced4fold}
	d_{il} = 
	\begin{pmatrix}
		0 & 0 & 0 & \chi_{xyz} & \chi_{xzx} & 0\\ 
		0 & 0 & 0 & \chi_{yzy} & \chi_{yzx} & 0\\ 
		\chi_{zxx} & \chi_{zyy} & \chi_{zzz} & 0 & 0 & 0
	\end{pmatrix} 
\end{equation}
with dependencies $\chi_{xyz} = -\chi_{yzx}$, $\chi_{yzy} = \chi_{xzx}$, and $\chi_{zxx} = \chi_{zyy}$.


\section{2-fold Rotational Symmetry}\label{sec:appendix:rotations:2foldrot}

In the case of 2-fold rotational symmetry around the z axis, the appropriate rotation matrix is given by equation~\ref{eq:background:NonlinearOptics:rotation:AllRotationMatrices} as
\begin{equation}\label{eq:piRotationMatrix}
	R(\theta=\pi)_{i,j} =
	\begin{bmatrix}
		-1 & 0 & 0\\ 
		0 & -1 & 0\\ 
		0 & 0 & 1
	\end{bmatrix}
\end{equation}
This corresponds to the coordinate substitution $x\rightarrow-x$, $y\rightarrow-y$, $z\rightarrow z$. Again, applying rotation to $\chi_{ijk}$ and enforcing the symmetry $\chi_{ijk}^{\prime}=\chi_{ijk}$ leaves the reduced tensor
\begin{equation}\label{eq:2foldChi}
	\chi^{(2)}_{ijk} =
	\begin{bmatrix}
		0 & 0 & 0 & \chi_{xyz} & \chi_{xzy} & 0 & 0 & \chi_{xxy} & \chi_{xyx}\\ 
		\chi_{yxx} & \chi_{yyy} & \chi_{yzz} & 0 & 0 & \chi_{yzx} & \chi_{yxz} & 0 & 0\\ 
		0 & 0 & 0 & \chi_{zyz} & \chi_{zzy} & 0 & 0 & \chi_{zxy} & \chi_{zyx}
	\end{bmatrix}
\end{equation}
with all remaining components left independent~\cite{Boyd2008a}. 

\section{3-fold Rotational Symmetry}\label{sec:appendix:rotations:3foldrot}

The case of 3-fold rotational symmetry is more complex, since for a rotation of $\theta=\frac{2}{3}\pi$ radians the rotation matrix is given by
\begin{equation}\label{eq:2pi/3RotationMatrix}
	R(\theta=\frac{2}{3}\pi)_{i,j} =
	\begin{bmatrix}
		-\frac{1}{2} & -\frac{\sqrt{3}}{2} & 0\\ 
		\frac{\sqrt{3}}{2} & -\frac{1}{2} & 0\\ 
		0 & 0 & 1
	\end{bmatrix}
\end{equation}
As before, we can rotate $\chi_{ijk}$ and equate to the initial tensor, giving
\begin{equation}\label{eq:RotateChi3fold}
	\chi^{\prime}_{ijk} =  
	R(\theta_{z})_{i\alpha} 
	R(\theta_{z})_{j\beta}
	R(\theta_{z})_{k\gamma}
	\chi^{(2)}_{\alpha \beta \gamma} =
	\chi_{ijk}
\end{equation}
This leaves the reduced tensor as
\begin{equation}\label{eq:3foldChi}
	\chi^{(2)}_{ijk} =
	\begin{bmatrix}
		\chi_{xxx} & \chi_{xyy} & 0 & \chi_{xyz} & \chi_{xzy} & \chi_{xzx} & \chi_{xxz} & \chi_{xxy} & \chi_{xyx}\\ 
		\chi_{yxx} & \chi_{yyy} & 0 & \chi_{yyz} & \chi_{yzy} & \chi_{yzx} & \chi_{yxz} & \chi_{yxy} & \chi_{yyx}\\ 
		\chi_{zxx} & \chi_{zyy} & \chi_{zzz} & 0 & 0 & 0 & 0 & \chi_{zxy} & \chi_{zyx}
	\end{bmatrix}
\end{equation}
with the dependencies 
\begin{equation}\label{eq:3foldDependancies}
\begin{split}
	&\chi_{xxx} = -\chi_{xyy} = -\chi_{yyz} = -\chi_{yxy}\\
	&\chi_{xyz} = -\chi_{yxz}, \chi_{xzy} = -\chi_{yzx}\\
	&\chi_{xzx} = \chi_{yzy}, \chi_{xxz} = \chi_{yyz}\\
	&\chi_{yyy} = -\chi_{yxx} = -\chi_{xxy} = -\chi_{xyx}\\
	&\chi_{zxx} = \chi_{zyy}, \chi_{zxy} = -\chi_{zyx}\\
	&\chi_{zzz}
\end{split}
\end{equation}
Under permutation symmetry, this reduces to
\begin{equation}\label{eq:Reduced3fold}
	d_{il} = 
	\begin{pmatrix}
		\chi_{xxx} & \chi_{xyy} & 0 & \chi_{xyz} & \chi_{xzx} & \chi_{xyx}\\ 
		\chi_{yxx} & \chi_{yyy} & 0 & \chi_{yzy} & \chi_{yzx} & \chi_{yxy}\\ 
		\chi_{zxx} & \chi_{zyy} & \chi_{zzz} & 0 & 0 & 0
	\end{pmatrix}
\end{equation}